@prefix :        <https://w3id.org/def/retele-share#> .
@prefix rdfs:    <http://www.w3.org/2000/01/rdf-schema#> .
@prefix dct:     <http://purl.org/dc/terms/> .
@prefix owl:     <http://www.w3.org/2002/07/owl#> .
@prefix xsd:     <http://www.w3.org/2001/XMLSchema#> .
@prefix rdf:     <http://www.w3.org/1999/02/22-rdf-syntax-ns#> .

<http://purl.org/net/def/metashare#CorpusImageInfo>
      a       owl:Class ;
      rdfs:comment "Groups together information on the image component of a resource."@en ;
      rdfs:label "corpus image info"@en , "información de las imágenes del corpus"@es .

<http://purl.org/net/def/metashare#address>
      a       owl:DatatypeProperty ;
      rdfs:domain
              [ a       owl:Class ;
                owl:unionOf (<http://purl.org/net/def/metashare#Organization> <http://purl.org/net/def/metashare#Person>)
              ] .

<http://purl.org/net/def/metashare#WordNet>
      a       owl:Class ;
      rdfs:label "WordNet"@en , "WordNet"@es ;
      rdfs:subClassOf <http://purl.org/net/def/metashare#LexicalConceptualResourceInfo> .

<http://purl.org/net/def/metashare#issn>
      a       owl:DatatypeProperty ;
      rdfs:domain <http://purl.org/net/def/metashare#DocumentInfo> .

<http://purl.org/net/def/metashare#AudioClassificationInfo>
      a       owl:Class ;
      rdfs:comment "Groups together information on audio type/genre of the resource."@en ;
      rdfs:label "audio classification info"@en , "información de la clasificación de los audios"@es .

<http://purl.org/net/def/metashare#languageDescriptionType>
      a       owl:ObjectProperty ;
      rdfs:label "language description type"@en , "tipo de gramática"@es ;
      rdfs:range <http://purl.org/net/def/metashare#LanguageDescriptionType> .

<http://purl.org/net/def/metashare#LinguisticInformation>
      a       owl:Class ;
      rdfs:comment "A more detailed account of the linguistic information contained in the lexical conceptual resource."@en , "linguistic information"@en ;
      rdfs:label "información lingüística"@es .

<http://purl.org/net/def/metashare#annotationManual>
      a       owl:ObjectProperty ;
      rdfs:comment "A bibliographic reference or ms:httpURI link to the annotation manual."@en ;
      rdfs:label "annotation manual"@en , "manual de anotación"@es ;
      rdfs:range <http://purl.org/net/def/metashare#Documentation> .

<http://purl.org/net/def/metashare#affiliation>
      a       owl:ObjectProperty ;
      rdfs:comment "Groups information on organization to whomtheperson is affiliated"@en ;
      rdfs:domain <http://purl.org/net/def/metashare#Person> ;
      rdfs:label "afiliación"@es , "affiliation"@en ;
      rdfs:range <http://purl.org/net/def/metashare#Organization> .

<http://purl.org/net/def/metashare#lexicalConceptualResourceVideoInfo>
      a       owl:ObjectProperty ;
      rdfs:domain <http://purl.org/net/def/metashare#LexicalConceptualResourceInfo> ;
      rdfs:label "lexical conceptual resource video info"@en , "información de los vídeos del recurso léxico conceptual"@es .

<http://purl.org/net/def/metashare#toolServiceInfo>
      a       owl:ObjectProperty ;
      rdfs:domain <http://purl.org/net/def/metashare#LanguageResource> .

<http://purl.org/net/def/metashare#LexicalConceptualResourceAudio>
      a       owl:Class ;
      rdfs:label "ficheros de audio del recurso léxico conceptual"@es , "lexical conceptual resource audio"@en ;
      rdfs:subClassOf <http://purl.org/net/def/metashare#LexicalConceptualResourceInfo> .

<http://purl.org/net/def/metashare#Project>
      a       owl:Class ;
      rdfs:label "proyecto"@es , "project"@en .

<http://purl.org/net/def/metashare#usageReport>
      a       owl:ObjectProperty ;
      rdfs:range <http://purl.org/net/def/metashare#Documentation> .

<http://xmlns.com/foaf/0.1/Actor>
      a       owl:Class ;
      rdfs:label "actor"@es .

<http://purl.org/net/def/metashare#distributionRightsHolder>
      a       owl:ObjectProperty ;
      rdfs:comment "Groups information on a person or an organization that holds the distribution rights. The range and scope of distribution rights is defined in the distribution agreement. The distributor in most cases only has a limited licence to distribute the work and collect royalties on behalf of the licensor or the IPR holder and cannot give to any recipient of the work permissions that exceed the scope of the distribution agreement (e.g. to allow uses of the work that are not defined in the distribution agreement)."@en ;
      rdfs:domain <http://purl.org/net/def/metashare#LicenceInfo> ;
      rdfs:label "propietario de los derechos de distribución"@es , "distribution rights holder"@en ;
      rdfs:range <http://purl.org/net/def/metashare#Actor> .

<https://w3id.org/def/retele-share>
      a       owl:Ontology ;
      rdfs:comment "Ontología para el Catálogo de Recursos Lingüísticos de ReTeLe (http://catalogo.retele.linkeddata.es/)  a partir de Metashare.owl (http://purl.org/net/def/metashare) "@es ;
      owl:versionInfo "1.0"@es .

<http://purl.org/net/def/metashare#relationInfo>
      a       owl:ObjectProperty ;
      rdfs:domain <http://purl.org/net/def/metashare#LanguageResource> .

<http://purl.org/net/def/metashare#departmentName>
      a       owl:DatatypeProperty ;
      rdfs:domain <http://purl.org/net/def/metashare#Organization> .

<http://purl.org/net/def/metashare#validationReport>
      a       owl:ObjectProperty ;
      rdfs:range <http://purl.org/net/def/metashare#Documentation> .

<http://purl.org/net/def/metashare#speechGenre>
      a       owl:DatatypeProperty ;
      rdfs:subPropertyOf <http://purl.org/net/def/metashare#genre> .

<http://purl.org/net/def/metashare#CharacterEncodingInfo>
      a       owl:Class ;
      rdfs:comment "Groups together information on character encoding of the resource."@en ;
      rdfs:label "character encoding info"@en , "información de la codificación de los caracteres"@es .

<http://purl.org/net/def/metashare#grammar>
      a       owl:NamedIndividual , <http://purl.org/net/def/metashare#LanguageDescriptionType> ;
      rdfs:label "grammar"@en , "gramática"@es .

<http://purl.org/net/def/metashare#resourceAssociatedWith>
      a       owl:DatatypeProperty ;
      rdfs:domain <http://purl.org/net/def/metashare#LanguageResource> .

<http://purl.org/net/def/metashare#lexicalConceptualResourceAudioInfo>
      a       owl:ObjectProperty ;
      rdfs:domain <http://purl.org/net/def/metashare#LexicalConceptualResourceInfo> ;
      rdfs:label "información de los ficheros de audio del recurso léxico conceptual"@es , "lexical conceptual resource audio info"@en .

<http://purl.org/net/def/metashare#LanguageDescriptionTextInfo>
      a       owl:Class ;
      rdfs:comment "Groups together all information relevant to the text module of a language description (e.g. format, languages, size etc.); it is obligatory for all language descriptions."@en ;
      rdfs:label "información de los textos de la gramática"@es , "language description text info"@en .

<http://purl.org/net/def/metashare#proprietary>
      a       <http://purl.org/net/def/metashare#LicenceInfo> , owl:NamedIndividual ;
      rdfs:label "propio"@es , "proprietary"@en .

<http://purl.org/net/def/metashare#executionLocation>
      a       owl:DatatypeProperty ;
      rdfs:domain <http://purl.org/net/def/metashare#LicenceInfo> .

<http://purl.org/net/def/metashare#faxNumber>
      a       owl:DatatypeProperty ;
      rdfs:domain
              [ a       owl:Class ;
                owl:unionOf (<http://purl.org/net/def/metashare#Organization> <http://purl.org/net/def/metashare#Person>)
              ] .

<http://purl.org/net/def/metashare#openForReuseWithRestrictions>
      a       <http://purl.org/net/def/metashare#License> , owl:NamedIndividual ;
      rdfs:label "open for reuse with restrictions"@en , "de uso abierto con restricciones"@es .

<http://purl.org/net/def/metashare#encodingLevel>
      a       owl:ObjectProperty ;
      rdfs:comment "Information on the contents of the lexicalConceptualResource as regards the linguistic level of analysis"@en ;
      rdfs:domain
              [ a       owl:Class ;
                owl:unionOf (<http://purl.org/net/def/metashare#LanguageDescriptionInfo> <http://purl.org/net/def/metashare#LexicalConceptualResourceInfo>)
              ] ;
      rdfs:label "nivel de codificación"@es , "ecoding level"@en ;
      rdfs:range
              [ a       owl:Class ;
                owl:unionOf (<http://purl.org/net/def/metashare#EncodingLevel>)
              ] .

<http://purl.org/net/def/metashare#CorpusAudioInfo>
      a       owl:Class ;
      rdfs:comment "Groups together information on the audio module of a corpus."@en ;
      rdfs:label "información de los ficheros de audio del corpus"@es , "corpus audio info"@en .

<http://purl.org/net/def/metashare#LexicalConceptualResourceImage>
      a       owl:Class ;
      rdfs:label "lexical conceptual resource image"@en , "imágenes del recurso léxico conceptual"@es ;
      rdfs:subClassOf <http://purl.org/net/def/metashare#LexicalConceptualResourceInfo> .

<http://purl.org/net/def/metashare#publications>
      a       owl:ObjectProperty ;
      rdfs:domain <http://purl.org/net/def/metashare#Actor> .

<http://purl.org/net/def/metashare#genre>
      a       owl:DatatypeProperty ;
      rdfs:domain <http://purl.org/net/def/metashare#ClassificationInfo> ;
      rdfs:range xsd:string .

<http://purl.org/net/def/metashare#CorpusInfo>
      a       owl:Class ;
      rdfs:comment "Groups together information on corpora of all media types."@en ;
      rdfs:label "corpus info"@en , "información del corpus"@es .

<http://purl.org/net/def/metashare#VideoClassificationInfo>
      a       owl:Class ;
      rdfs:comment "Groups together information on video genre of the resource."@en ;
      rdfs:label "información de la clasificación de los vídeos"@es , "video classification info"@en .

<http://purl.org/net/def/metashare#videoGenre>
      a       owl:DatatypeProperty ;
      rdfs:subPropertyOf <http://purl.org/net/def/metashare#genre> .

<http://purl.org/net/def/metashare#ImageClassificationInfo>
      a       owl:Class ;
      rdfs:comment "Groups information on the classification of the image corpus."@en ;
      rdfs:label "image classification info"@en , "información de la clasificación de las imágenes"@es .

<http://purl.org/net/def/metashare#LanguageVarietyInfo>
      a       owl:Class ;
      rdfs:comment "Groups information on language varieties occurred in the resource (e.g. dialects)."@en ;
      rdfs:label "información de las variedades del lenguaje"@es , "language variety info"@en .

<http://purl.org/net/def/metashare#zipCode>
      a       owl:DatatypeProperty ;
      rdfs:domain
              [ a       owl:Class ;
                owl:unionOf (<http://purl.org/net/def/metashare#Organization> <http://purl.org/net/def/metashare#Person>)
              ] .

<http://purl.org/net/def/metashare#email>
      a       owl:DatatypeProperty ;
      rdfs:comment "The email address of a person or an organization"@en ;
      rdfs:domain
              [ a       owl:Class ;
                owl:unionOf (<http://purl.org/net/def/metashare#Organization> <http://purl.org/net/def/metashare#Person>)
              ] ;
      rdfs:range xsd:string .

<http://purl.org/net/def/metashare#originalSource>
      a       owl:DatatypeProperty ;
      rdfs:domain
              [ a       owl:Class ;
                owl:unionOf (<http://purl.org/net/def/metashare#CorpusAudioInfo> <http://purl.org/net/def/metashare#CorpusImageInfo> <http://purl.org/net/def/metashare#CorpusTextInfo> <http://purl.org/net/def/metashare#CorpusTextNgramInfo> <http://purl.org/net/def/metashare#CorpusTextNumericalInfo> <http://purl.org/net/def/metashare#CorpusVideoInfo> <http://purl.org/net/def/metashare#LanguageDescriptionImageInfo> <http://purl.org/net/def/metashare#LanguageDescriptionInfo> <http://purl.org/net/def/metashare#LanguageDescriptionTextInfo> <http://purl.org/net/def/metashare#LanguageDescriptionVideoInfo> <http://purl.org/net/def/metashare#LexicalConceptualResourceInfo> <http://purl.org/net/def/metashare#ToolServiceInfo>)
              ] .

<http://purl.org/net/def/metashare#LanguageInfo>
      a       owl:Class ;
      rdfs:comment "Groups information on the languages represented in the resource"@en ;
      rdfs:label "language info"@en , "información de las lenguas del recurso"@es .

<http://purl.org/net/def/metashare#LexicalConceptualResourceVideoInfo>
      a       owl:Class ;
      rdfs:comment "Groups information on the video part of the lexical conceptual resource."@en ;
      rdfs:label "lexical conceptual resource video info"@en , "información de los vídeos del recurso léxico conceptual"@es , "información audiovisual del recurso léxico conceptual"@es .

<http://purl.org/net/def/metashare#fundingProject>
      a       owl:ObjectProperty ;
      rdfs:comment "Groups information on the project that has funded the resource"@en ;
      rdfs:domain <http://purl.org/net/def/metashare#LanguageResource> ;
      rdfs:label "funding project"@en , "proyecto financiador"@es ;
      rdfs:range <http://purl.org/net/def/metashare#Project> .

<http://purl.org/net/def/metashare#LanguageVarietyType>
      a       owl:Class ;
      rdfs:comment "Specifies the type of the language variety that occurs in the resource or is supported by a tool/service."@en ;
      rdfs:label "language variety type"@en , "tipo de variedad de la lengua"@es .

<http://purl.org/net/def/metashare#userNature>
      a       owl:ObjectProperty ;
      rdfs:domain <http://purl.org/net/def/metashare#LicenceInfo> .

<http://purl.org/net/def/metashare#url>
      a       owl:DatatypeProperty ;
      rdfs:comment "A URL used as homepage of an entity (e.g. of a person, organization, resource etc.) and/or where an entity (e.g.LR, document etc.) is located"@en ;
      rdfs:domain
              [ a       owl:Class ;
                owl:unionOf (<http://purl.org/net/def/metashare#LanguageResource> <http://purl.org/net/def/metashare#Organization> <http://purl.org/net/def/metashare#Person> <http://purl.org/net/def/metashare#Project>)
              ] ;
      rdfs:range xsd:string .

<http://purl.org/net/def/metashare#extratextualInformation>
      a       owl:ObjectProperty ;
      rdfs:comment "An indication of the extratextual information contained in the lexicalConceptualResouce; can be used as an alternative to audio, image, videos etc. for cases where these are not considered an important part of the lcr."@en ;
      rdfs:domain <http://purl.org/net/def/metashare#LexicalConceptualResourceInfo> ;
      rdfs:label "extra textual information"@en , "información no textual"@es .

<http://purl.org/net/def/metashare#size>
      a       owl:DatatypeProperty ;
      rdfs:comment "Specifies the size of the resource with regard to the SizeUnit measurement in form of a number"@en ;
      rdfs:domain <http://purl.org/net/def/metashare#Size> ;
      rdfs:range xsd:string .

<http://purl.org/net/def/metashare#lexicalConceptualResourceMediaPartInfo>
      a       owl:ObjectProperty ;
      rdfs:domain <http://purl.org/net/def/metashare#LexicalConceptualResourceInfo> ;
      rdfs:label "lexical conceptual resource media part info"@en , "información de la parte multimedia del recurso léxico conceptual"@es .

<http://purl.org/net/def/metashare#metaShareId>
      a       owl:DatatypeProperty ;
      rdfs:domain <http://purl.org/net/def/metashare#LanguageResource> .

<http://purl.org/net/def/metashare#InputInfo>
      a       owl:Class ;
      rdfs:comment "Groups together information on the requirements set on the input resource of a tool or service."@en ;
      rdfs:label "información de los requisitos de entrada"@es , "información de entrada"@es , "input info"@en .

<http://purl.org/net/def/metashare#Organization>
      a       owl:Class ;
      owl:equivalentClass <http://xmlns.com/foaf/0.1/Organization> .

<http://purl.org/net/def/metashare#accessTool>
      a       owl:DatatypeProperty ;
      rdfs:domain <http://purl.org/net/def/metashare#LanguageResource> .

<http://purl.org/net/def/metashare#corpusInfo>
      a       owl:ObjectProperty ;
      rdfs:domain <http://purl.org/net/def/metashare#LanguageResource> ;
      rdfs:label "corpus info"@en , "Groups together information on corpora of all media types."@en , "información del corpus"@es .

<http://purl.org/net/def/metashare#characterEncodingInfo>
      a       owl:ObjectProperty ;
      rdfs:comment "Groups together information on character encoding of the resource"@en ;
      rdfs:domain
              [ a       owl:Class ;
                owl:unionOf (<http://purl.org/net/def/metashare#CorpusTextInfo> <http://purl.org/net/def/metashare#CorpusTextNgramInfo> <http://purl.org/net/def/metashare#LanguageDescriptionTextInfo> <http://purl.org/net/def/metashare#LexicalConceptualResourceTextInfo>)
              ] ;
      rdfs:label "información de codificación de caracteres"@es , "character encoding info"@en ;
      rdfs:range
              [ a       owl:Class ;
                owl:unionOf (<http://purl.org/net/def/metashare#CharacterEncodingInfo>)
              ] .

<http://purl.org/net/def/metashare#TextClassificationInfo>
      a       owl:Class ;
      rdfs:comment "Groups together information on text type/genre of the resource."@en ;
      rdfs:label "información de la clasificación de los textos"@es , "text classification info"@en .

<http://purl.org/net/def/metashare#metadataSource>
      a       owl:DatatypeProperty ;
      rdfs:domain <http://purl.org/net/def/metashare#LanguageResource> .

<http://purl.org/net/def/metashare#creationTool>
      a       owl:DatatypeProperty ;
      rdfs:domain
              [ a       owl:Class ;
                owl:unionOf (<http://purl.org/net/def/metashare#CorpusAudioInfo> <http://purl.org/net/def/metashare#CorpusImageInfo> <http://purl.org/net/def/metashare#CorpusTextInfo> <http://purl.org/net/def/metashare#CorpusTextNgramInfo> <http://purl.org/net/def/metashare#CorpusTextNumericalInfo> <http://purl.org/net/def/metashare#CorpusVideoInfo> <http://purl.org/net/def/metashare#LanguageDescriptionImageInfo> <http://purl.org/net/def/metashare#LanguageDescriptionInfo> <http://purl.org/net/def/metashare#LanguageDescriptionTextInfo> <http://purl.org/net/def/metashare#LanguageDescriptionVideoInfo> <http://purl.org/net/def/metashare#LexicalConceptualResourceInfo>)
              ] .

<http://purl.org/net/def/metashare#textFormatInfo>
      a       owl:ObjectProperty ;
      rdfs:comment "Groups information on the text format(s) of a resource"@en ;
      rdfs:domain
              [ a       owl:Class ;
                owl:unionOf (<http://purl.org/net/def/metashare#CorpusTextInfo> <http://purl.org/net/def/metashare#CorpusTextNgramInfo> <http://purl.org/net/def/metashare#LanguageDescriptionTextInfo> <http://purl.org/net/def/metashare#LexicalConceptualResourceTextInfo>)
              ] ;
      rdfs:range
              [ a       owl:Class ;
                owl:unionOf (<http://purl.org/net/def/metashare#TextFormatInfo>)
              ] .

:islrn
      a       owl:DatatypeProperty ;
      rdfs:domain <http://purl.org/net/def/metashare#LanguageResource> ;
      rdfs:label "International Standard Language Resource Number"@en , "ISLRN"@en .

<http://purl.org/net/def/metashare#CorpusTextNumericalInfo>
      a       owl:Class ;
      rdfs:label "Groups together information on the textNumerical component of a corpus. It is used basically for the textual representation of measurements and observations linked to sensorimotor recordings."@en , "corpus text numerical info"@en , "información numérica de los textos del corpus"@es .

<http://purl.org/net/def/metashare#creationMode>
      a       owl:ObjectProperty ;
      rdfs:comment "Specifies whether the resource is created automatically or in manual or interactive mode."@en ;
      rdfs:domain
              [ a       owl:Class ;
                owl:unionOf (<http://purl.org/net/def/metashare#CorpusAudioInfo> <http://purl.org/net/def/metashare#CorpusImageInfo> <http://purl.org/net/def/metashare#CorpusTextInfo> <http://purl.org/net/def/metashare#CorpusTextNgramInfo> <http://purl.org/net/def/metashare#CorpusTextNumericalInfo> <http://purl.org/net/def/metashare#CorpusVideoInfo> <http://purl.org/net/def/metashare#LanguageDescriptionImageInfo> <http://purl.org/net/def/metashare#LanguageDescriptionInfo> <http://purl.org/net/def/metashare#LanguageDescriptionTextInfo> <http://purl.org/net/def/metashare#LanguageDescriptionVideoInfo> <http://purl.org/net/def/metashare#LexicalConceptualResourceInfo>)
              ] ;
      rdfs:label "modo de creación"@es , "creation mode"@en .

<http://purl.org/net/def/metashare#FrameNet>
      a       owl:Class ;
      rdfs:label "FrameNet"@en , "FrameNet"@es ;
      rdfs:subClassOf <http://purl.org/net/def/metashare#LexicalConceptualResourceInfo> .

<http://purl.org/net/def/metashare#audioGenre>
      a       owl:DatatypeProperty ;
      rdfs:subPropertyOf <http://purl.org/net/def/metashare#genre> .

<http://purl.org/net/def/metashare#LingualityType>
      a       owl:Class ;
      rdfs:comment "clasificación por número de lenguas"@es , "Indicates whether the resource includes one, two or more languages."@en ;
      rdfs:label "linguality type"@en .

<http://purl.org/net/def/metashare#Corpus>
      a       owl:Class ;
      rdfs:label "corpus"@en , "corpus"@es ;
      rdfs:subClassOf <http://purl.org/net/def/metashare#LanguageResource> ;
      owl:equivalentClass
              [ a       owl:Restriction ;
                owl:onProperty <http://purl.org/net/def/metashare#corpusInfo> ;
                owl:someValuesFrom <http://purl.org/net/def/metashare#CorpusInfo>
              ] .

<http://purl.org/net/def/metashare#documentation>
      a       owl:ObjectProperty ;
      rdfs:domain <http://purl.org/net/def/metashare#LanguageResource> ;
      rdfs:label "documentación"@es , "documentation"@en ;
      rdfs:range <http://purl.org/net/def/metashare#Documentation> .

<http://purl.org/net/def/metashare#other>
      a       <http://purl.org/net/def/metashare#LicenceInfo> , owl:NamedIndividual , <http://purl.org/net/def/metashare#LanguageDescriptionType> ;
      rdfs:label "otro"@es , "other"@en .

<http://purl.org/net/def/metashare#MachineReadableDictionary>
      a       owl:Class ;
      rdfs:label "diccionario electrónico"@es , "machine readable dictionary"@en ;
      rdfs:subClassOf <http://purl.org/net/def/metashare#LexicalConceptualResourceInfo> .

<http://purl.org/net/def/metashare#sizeUnit>
      a       owl:ObjectProperty ;
      rdfs:comment "Specifies the unit that is used when providing information on the size of the resource or of resource parts"@en ;
      rdfs:domain <http://purl.org/net/def/metashare#Size> ;
      rdfs:range <http://purl.org/net/def/metashare#SizeUnit> .

<http://purl.org/net/def/metashare#creationEndDate>
      a       owl:DatatypeProperty ;
      rdfs:comment "The date in which the creation process was completed"@en ;
      rdfs:domain <http://purl.org/net/def/metashare#LanguageResource> ;
      rdfs:range xsd:date .

<http://purl.org/net/def/metashare#ComputationalLexicon>
      a       owl:Class ;
      rdfs:label "computational lexicon"@en , "lexicón computacional"@es ;
      rdfs:subClassOf <http://purl.org/net/def/metashare#LexicalConceptualResourceInfo> .

<http://www.w3.org/ns/dcat#Dataset>
      a       owl:Class ;
      rdfs:label "conjunto de datos"@es .

<http://purl.org/net/def/metashare#recorder>
      a       owl:ObjectProperty ;
      rdfs:range
              [ a       owl:Class ;
                owl:unionOf (<http://purl.org/net/def/metashare#Actor>)
              ] .

<http://purl.org/net/def/metashare#Documentation>
      a       owl:Class ;
      rdfs:comment "Refers to papers, manuals, reports etc. describing the resource"@en ;
      rdfs:label "documentación"@es , "documentation"@en .

<http://purl.org/net/def/metashare#region>
      a       owl:DatatypeProperty ;
      rdfs:domain
              [ a       owl:Class ;
                owl:unionOf (<http://purl.org/net/def/metashare#Organization> <http://purl.org/net/def/metashare#Person>)
              ] .

<http://purl.org/net/def/metashare#LanguageDescription>
      a       owl:Class ;
      rdfs:label "language description"@en , "gramática"@es ;
      rdfs:subClassOf <http://purl.org/net/def/metashare#LanguageResource> .

<http://purl.org/net/def/metashare#languageVarietyType>
      a       owl:ObjectProperty ;
      rdfs:comment "Specifies the type of the language variety that occurs in the resource or is supported by a tool/service"@en ;
      rdfs:domain <http://purl.org/net/def/metashare#LanguageVarietyInfo> ;
      rdfs:label "language variety type"@en , "tipo de variedad de la lengua"@es ;
      rdfs:range <http://purl.org/net/def/metashare#LanguageVarietyType> .

<http://purl.org/net/def/metashare#LexicalConceptualResourceImageInfo>
      a       owl:Class ;
      rdfs:comment "Groups information on the image part of the lexical/conceptual resource."@en ;
      rdfs:label "lexical conceptual resource image info"@en , "información de las imágenes del recurso léxico conceptual"@es .

<http://purl.org/net/def/metashare#DomainInfo>
      a       owl:Class ;
      rdfs:comment "Groups together information on domains represented in the resource; can be repeated for parts of the resource with distinct domain"@en ;
      rdfs:label "información del dominio"@es , "domain info"@en .

<http://purl.org/net/def/metashare#evaluationReport>
      a       owl:ObjectProperty ;
      rdfs:comment "A bibliographical record of or link to a report describing the evaluation process, tool, method etc. of the tool or service."@en ;
      rdfs:label "informe de evaluación"@es , "evaluation record"@en ;
      rdfs:range <http://purl.org/net/def/metashare#Documentation> .

<http://purl.org/net/def/metashare#sizePerDomain>
      a       owl:ObjectProperty ;
      rdfs:domain <http://purl.org/net/def/metashare#DomainInfo> .

<http://purl.org/net/def/metashare#LexicalConceptualResourceTextInfo>
      a       owl:Class ;
      rdfs:comment "Groups information on the textual part of the lexical/conceptual resource."@en ;
      rdfs:label "lexical conceptual resource text info"@en , "información de los textos del recurso léxico conceptual"@es .

<http://purl.org/net/def/metashare#LexicalConceptualResourceVideo>
      a       owl:Class ;
      rdfs:label "lexical conceptual resource video"@en , "vídeos del recurso léxico conceptual"@es ;
      rdfs:subClassOf <http://purl.org/net/def/metashare#LexicalConceptualResourceInfo> .

<http://purl.org/net/def/metashare#TerminologicalResource>
      a       owl:Class ;
      rdfs:label "terminological resource"@en , "recurso terminológico"@es ;
      rdfs:subClassOf <http://purl.org/net/def/metashare#LexicalConceptualResourceInfo> .

<http://purl.org/net/def/metashare#revision>
      a       owl:DatatypeProperty ;
      rdfs:domain
              [ a       owl:Class ;
                owl:unionOf (<http://purl.org/net/def/metashare#LanguageResource> <http://purl.org/net/def/metashare#MetadataInfo>)
              ] .

xsd:date
      a       rdfs:Datatype .

<http://purl.org/net/def/metashare#LicenseCategory>
      a       owl:Class ;
      rdfs:comment "A way of classifying licences according to their conditions of use (CLARIN recommendation)"@en ;
      rdfs:label "categorización de las licencias"@es , "license category"@en .

<http://purl.org/net/def/metashare#Person>
      a       owl:Class ;
      rdfs:label "person"@en , "persona"@es .

<http://purl.org/net/def/metashare#lexicalConceptualResourceInfo>
      a       owl:ObjectProperty ;
      rdfs:domain <http://purl.org/net/def/metashare#LanguageResource> ;
      rdfs:label "lexical conceptual resource info"@en , "información del recurso léxico conceptual"@es ;
      rdfs:range <http://purl.org/net/def/metashare#LexicalConceptualResourceInfo> .

<http://purl.org/net/def/metashare#LanguageDescriptionImageInfo>
      a       owl:Class ;
      rdfs:comment "Groups together all information relevant to the image module of a language description (e.g. format, languages, size etc.), if there are any (e.g. for sign language grammars)."@en ;
      rdfs:label "language description image info"@en , "información de las imágenes de las gramáticas"@es .

<http://purl.org/net/def/metashare#actualUseInfo>
      a       owl:ObjectProperty ;
      rdfs:comment "Groups information on how the resource has already been used."@en ;
      rdfs:domain <http://purl.org/net/def/metashare#LanguageResource> ;
      rdfs:label "actual use info"@en , "información de uso"@es .

<http://purl.org/net/def/metashare#extraTextualInformationUnit>
      a       owl:ObjectProperty ;
      rdfs:comment "The unit of the extratextual information contained in the lexical conceptual resource."@en ;
      rdfs:domain <http://purl.org/net/def/metashare#LexicalConceptualResourceInfo> ;
      rdfs:label "unidad de información no textual"@es , "extra textual information unit"@en .

<http://purl.org/net/def/metashare#Ontology>
      a       owl:Class ;
      rdfs:label "ontología"@es , "ontology"@en ;
      rdfs:subClassOf <http://purl.org/net/def/metashare#LexicalConceptualResourceInfo> .

<http://purl.org/net/def/metashare#LexicalConceptualResourceAudioInfo>
      a       owl:Class ;
      rdfs:comment "Groups information on the audio part of the lexical/conceptual resource."@en ;
      rdfs:label "información de los ficheros de audio del recurso léxico conceptual"@es , "lexical conceptual resource audio info"@en .

<http://purl.org/net/def/metashare#AnnotationInfo>
      a       owl:Class ;
      rdfs:comment "Groups information on the annotated part(s) of a resource."@en ;
      rdfs:label "informacion de las anotaciones"@es , "annotation info"@en .

<http://purl.org/net/def/metashare#fee>
      a       owl:DatatypeProperty ;
      rdfs:domain <http://purl.org/net/def/metashare#LicenceInfo> .

<http://purl.org/net/def/metashare#LanguageDescriptionVideoInfo>
      a       owl:Class ;
      rdfs:comment "Groups together all information relevant to the video parts of a language description (e.g. format, languages, size etc.), if there are any (e.g. for sign language grammars)."@en ;
      rdfs:label "información de los vídeos de la gramática"@es , "language description video info"@en .

<http://purl.org/net/def/metashare#attributionText>
      a       owl:DatatypeProperty ;
      rdfs:domain <http://purl.org/net/def/metashare#LicenceInfo> .

<http://purl.org/net/def/metashare#languageInfo>
      a       owl:ObjectProperty ;
      rdfs:comment "Groups information on the languages represented in the resource"@en ;
      rdfs:domain
              [ a       owl:Class ;
                owl:unionOf (<http://purl.org/net/def/metashare#CorpusAudioInfo> <http://purl.org/net/def/metashare#CorpusImageInfo> <http://purl.org/net/def/metashare#CorpusTextInfo> <http://purl.org/net/def/metashare#CorpusTextNgramInfo> <http://purl.org/net/def/metashare#CorpusVideoInfo> <http://purl.org/net/def/metashare#LanguageDescriptionImageInfo> <http://purl.org/net/def/metashare#LanguageDescriptionTextInfo> <http://purl.org/net/def/metashare#LanguageDescriptionVideoInfo> <http://purl.org/net/def/metashare#LexicalConceptualResourceAudioInfo> <http://purl.org/net/def/metashare#LexicalConceptualResourceImageInfo> <http://purl.org/net/def/metashare#LexicalConceptualResourceTextInfo> <http://purl.org/net/def/metashare#LexicalConceptualResourceVideoInfo>)
              ] ;
      rdfs:label "language info"@en , "información de las lenguas del recurso"@es ;
      rdfs:range
              [ a       owl:Class ;
                owl:unionOf (<http://purl.org/net/def/metashare#LanguageInfo>)
              ] .

<http://purl.org/net/def/metashare#conditionsOfUse>
      a       owl:ObjectProperty ;
      rdfs:domain <http://purl.org/net/def/metashare#LicenceInfo> ;
      rdfs:label "conditions of use"@en , "condiciones de uso"@es .

<http://purl.org/net/def/metashare#country>
      a       owl:DatatypeProperty ;
      rdfs:domain
              [ a       owl:Class ;
                owl:unionOf (<http://purl.org/net/def/metashare#Organization> <http://purl.org/net/def/metashare#Person>)
              ] .

<http://purl.org/net/def/metashare#annotator>
      a       owl:ObjectProperty ;
      rdfs:comment "Groups information on the annotators of the specific annotation type."@en ;
      rdfs:label "anotador"@es , "annotator"@en ;
      rdfs:range <http://purl.org/net/def/metashare#Actor> .

<http://purl.org/net/def/metashare#resourceShortName>
      a       owl:DatatypeProperty ;
      rdfs:comment "The short form (abbreviation, acronym etc.) used to identify the resource; the element can be repeated for the different language versions using the \"lang\" attribute to specify the language."@en ;
      rdfs:domain <http://purl.org/net/def/metashare#LanguageResource> ;
      rdfs:range rdf:langString .

<http://purl.org/net/def/metashare#membershipInfo>
      a       owl:ObjectProperty ;
      rdfs:domain <http://purl.org/net/def/metashare#LicenceInfo> .

<http://purl.org/net/def/metashare#MetadataInfo>
      a       owl:Class ;
      rdfs:comment "Groups information on the metadata record itself."@en ;
      rdfs:label "metadata info"@en , "información de los metadatos"@es .

<http://purl.org/net/def/metashare#foreseenUseInfo>
      a       owl:ObjectProperty ;
      rdfs:comment "Groups information on the use for which the resource is created."@en ;
      rdfs:domain <http://purl.org/net/def/metashare#LanguageResource> ;
      rdfs:label "foreseen use info"@en , "información del uso previsto del recurso"@es .

<http://purl.org/net/def/metashare#organizationInfo>
      a       owl:ObjectProperty ;
      rdfs:domain <http://purl.org/net/def/metashare#Actor> ;
      rdfs:range <http://purl.org/net/def/metashare#Organization> .

<http://purl.org/net/def/metashare#LanguageResource>
      a       owl:Class ;
      rdfs:label "language resource"@en , "recurso lingüístico"@es ;
      dct:replaces <http://www.ilsp.gr/META-XMLSchema#resourceInfo> ;
      owl:equivalentClass <http://www.w3.org/ns/dcat#Dataset> .

<http://purl.org/net/def/metashare#imageGenre>
      a       owl:DatatypeProperty ;
      rdfs:subPropertyOf <http://purl.org/net/def/metashare#genre> .

<http://purl.org/net/def/metashare#TextFormatInfo>
      a       owl:Class ;
      rdfs:comment "Groups information on the text format(s) of a resource."@en ;
      rdfs:label "información de los formatos del texto"@es , "text format info"@en .

<http://purl.org/net/def/metashare#LicenceInfo>
      a       owl:Class ;
      rdfs:comment "Groups information on licences for the resource; can be repeated to allow for different modes of access and restrictions of use (e.g. free for academic use, on-a-fee basis for commercial use, download of a sample for free use etc.)"@en ;
      rdfs:label "licence info"@en , "información de la licencia del recurso"@es .

<http://purl.org/net/def/metashare#sizePerLanguage>
      a       owl:ObjectProperty ;
      rdfs:domain <http://purl.org/net/def/metashare#LanguageInfo> .

<http://purl.org/net/def/metashare#city>
      a       owl:DatatypeProperty ;
      rdfs:domain
              [ a       owl:Class ;
                owl:unionOf (<http://purl.org/net/def/metashare#Organization> <http://purl.org/net/def/metashare#Person>)
              ] .

<http://purl.org/net/def/metashare#lexicalConceptualResourceTextInfo>
      a       owl:ObjectProperty ;
      rdfs:domain <http://purl.org/net/def/metashare#LexicalConceptualResourceInfo> ;
      rdfs:label "lexical conceptual resource text info"@en , "información de los textos del recurso léxico conceptual"@es .

<http://purl.org/net/def/metashare#updateFrequency>
      a       owl:DatatypeProperty ;
      rdfs:domain <http://purl.org/net/def/metashare#LanguageResource> .

<http://purl.org/net/def/metashare#languageVarietyInfo>
      a       owl:ObjectProperty ;
      rdfs:comment "Groups information on language varieties occurred in the resource (e.g. dialects)"@en ;
      rdfs:domain <http://purl.org/net/def/metashare#LanguageInfo> ;
      rdfs:label "información de las variedades del recurso"@es , "language variety info"@en ;
      rdfs:range <http://purl.org/net/def/metashare#LanguageVarietyInfo> .

<http://purl.org/net/def/metashare#personInfo>
      a       owl:ObjectProperty ;
      rdfs:domain <http://purl.org/net/def/metashare#Actor> .

<http://purl.org/net/def/metashare#OutputInfo>
      a       owl:Class ;
      rdfs:comment "Groups together information on the requirements set on the output of a tool or service."@en ;
      rdfs:label "información de los requisitos de salida"@es , "información de salida"@es , "output info"@en .

<http://purl.org/net/def/metashare#validator>
      a       owl:ObjectProperty ;
      rdfs:range <http://purl.org/net/def/metashare#Actor> .

<http://purl.org/net/def/metashare#iprHolder>
      a       owl:ObjectProperty ;
      rdfs:comment "Groups information on a person or an organization who holds the full Intellectual Property Rights (Copyright, trademark etc) that subsist in the resource. The IPR holder could be different from the creator that may have assigned the rights to the IPR holder (e.g. an author as a creator assigns her rights to the publisher who is the IPR holder) and the distributor that holds a specific licence (i.e. a permission) to distribute the work within the META-SHARE network."@en , "A person or an organization who holds the full Intellectual Property Rights (Copyright, trademark etc) that subsist in the resource. The IPR holder could be different from the creator that may have assigned the rights to the IPR holder (e.g. an author as a creator assigns her rights to the publisher who is the IPR holder) and the distributor that holds a specific licence (i.e. a permission) to distribute the work via a specific distributor."@en ;
      rdfs:label "titular de DPI"@es , "IPR holder"@en ;
      rdfs:range <http://purl.org/net/def/metashare#Actor> .

<http://purl.org/net/def/metashare#organizationShortName>
      a       owl:DatatypeProperty ;
      rdfs:domain <http://purl.org/net/def/metashare#Organization> .

<http://purl.org/net/def/metashare#toolDocumentationType>
      a       owl:ObjectProperty ;
      rdfs:domain <http://purl.org/net/def/metashare#LanguageResource> .

<http://purl.org/net/def/metashare#CharacterEncoding>
      a       owl:Class ;
      rdfs:comment "The name of the character encoding used in the resource or accepted by the tool/service."@en ;
      rdfs:label "codificación de los caracteres"@es , "character encoding"@en .

<http://purl.org/net/def/metashare#ToolServiceInfo>
      a       owl:Class ;
      rdfs:comment "Groups together elements required for the description of tools and services."@en ;
      rdfs:label "información de herramientas y servicios"@es , "tool service info"@en .

<http://purl.org/net/def/metashare#CorpusTextInfo>
      a       owl:Class ;
      rdfs:comment "Groups together information on the text component of a resource."@en , "corpus text info"@en ;
      rdfs:label "información de los textos del corpus"@es .

<http://purl.org/net/def/metashare#distributionAccessMedium>
      a       owl:ObjectProperty ;
      rdfs:comment "Specifies the medium (channel) used for delivery or providing access to the resource."@en ;
      rdfs:domain <http://purl.org/net/def/metashare#LanguageResource> ;
      rdfs:label "medio de acceso o distribución"@es , "distribution access medium"@en .

<http://purl.org/net/def/metashare#EncodingLevel>
      a       owl:Class ;
      rdfs:comment "Information on the linguistic levels covered by the resource (grammar or lexical/conceptual resource)."@en ;
      rdfs:label "nivel de codificación"@es , "encoding level"@en .

<http://purl.org/net/def/metashare#ContactPerson>
      a       owl:Class ;
      rdfs:comment "Groups information on the person(s) that is/are responsible for providing further information regarding the resource"@en ;
      rdfs:label "persona de contacto"@es , "contact person"@en .

<http://purl.org/net/def/metashare#DocumentInfo>
      a       owl:Class ;
      rdfs:comment "document info"@en , "Groups information on all the documents reporting on various aspects of the resource (creation, usage etc.), published or unpublished; it is used in various places of the metadata schema depending on its role (e.g. usage report, validation report, annotation manual etc.)."@en ;
      rdfs:label "información de la documentación"@es .

<http://purl.org/net/def/metashare#documentUnstructured>
      a       owl:DatatypeProperty ;
      rdfs:domain <http://purl.org/net/def/metashare#Documentation> .

<http://purl.org/net/def/metashare#Lexicon>
      a       owl:Class ;
      rdfs:label "lexicón"@es , "lexicon"@en ;
      rdfs:subClassOf <http://purl.org/net/def/metashare#LexicalConceptualResourceInfo> .

<http://purl.org/net/def/metashare#Size>
      a       owl:Class ;
      rdfs:label "size"@en , "tamaño"@es .

<http://purl.org/net/def/metashare#languageDescriptionInfo>
      a       owl:ObjectProperty ;
      rdfs:domain <http://purl.org/net/def/metashare#LanguageResource> ;
      rdfs:label "language description info"@en , "información de la gramática"@es .

<http://purl.org/net/def/metashare#evaluator>
      a       owl:ObjectProperty ;
      rdfs:comment "Groups information on person or organization that evaluated the tool or service."@en ;
      rdfs:label "evaluador"@es , "evaluator"@en ;
      rdfs:range <http://purl.org/net/def/metashare#Actor> .

<http://purl.org/net/def/metashare#underNegotiation>
      a       <http://purl.org/net/def/metashare#LicenceInfo> , owl:NamedIndividual ;
      rdfs:label "under Negotiation"@en , "objeto de negociación"@es .

<http://purl.org/net/def/metashare#License>
      a       owl:Class ;
      rdfs:comment "The license of use for the resource."@en ;
      rdfs:label "license"@en , "licencia"@es .

<http://purl.org/net/def/metashare#conformanceToClassificationScheme>
      a       owl:ObjectProperty ;
      rdfs:comment "Specifies the external classification schemes."@en ;
      rdfs:domain
              [ a       owl:Class ;
                owl:unionOf (<http://purl.org/net/def/metashare#AudioClassificationInfo> <http://purl.org/net/def/metashare#DomainInfo> <http://purl.org/net/def/metashare#ImageClassificationInfo> <http://purl.org/net/def/metashare#TextClassificationInfo> <http://purl.org/net/def/metashare#VideoClassificationInfo>)
              ] ;
      rdfs:label "según esquema de clasificación"@es , "conformance to classification scheme"@en .

<http://purl.org/net/def/metashare#userManual>
      a       owl:ObjectProperty ;
      rdfs:domain <http://purl.org/net/def/metashare#LanguageResource> ;
      rdfs:range <http://purl.org/net/def/metashare#DocumentInfo> .

<http://purl.org/net/def/metashare#LexicalConceptualResourceText>
      a       owl:Class ;
      rdfs:label "textos del recurso léxico conceptual"@es , "lexical conceptual resource text"@en ;
      rdfs:subClassOf <http://purl.org/net/def/metashare#LexicalConceptualResourceInfo> .

<http://xmlns.com/foaf/0.1/Organization>
      a       owl:Class ;
      rdfs:label "organización"@es , "organization"@en .

<http://purl.org/net/def/metashare#CorpusTextNgramInfo>
      a       owl:Class ;
      rdfs:comment "Groups together information required for n-gram resources; information can be provided both as regards features drawn from the source corpus (e.g. language coverage, size, format, domains etc.) and features pertaining to the n-gram output itself (e.g. range of n-grams, type of item included, etc.)."@en ;
      rdfs:label "corpus text ngram info"@en , "información de los n-gramas de los textos del corpus"@es .

<http://purl.org/net/def/metashare#creationStartDate>
      a       owl:DatatypeProperty ;
      rdfs:comment "The date in which the creation process was started"@en ;
      rdfs:domain <http://purl.org/net/def/metashare#LanguageResource> ;
      rdfs:range xsd:date .

<http://purl.org/net/def/metashare#lexicalConceptualResourceImageInfo>
      a       owl:ObjectProperty ;
      rdfs:domain <http://purl.org/net/def/metashare#LexicalConceptualResourceInfo> ;
      rdfs:label "lexical conceptual resource image info"@en , "información de las imágenes del recurso léxico conceptual"@es .

<http://purl.org/net/def/metashare#domainInfo>
      a       owl:ObjectProperty ;
      rdfs:comment "Groups together information on domains represented in the resource; can be repeated for parts of the resource with distinct domain"@en ;
      rdfs:domain
              [ a       owl:Class ;
                owl:unionOf (<http://purl.org/net/def/metashare#CorpusAudioInfo> <http://purl.org/net/def/metashare#CorpusImageInfo> <http://purl.org/net/def/metashare#CorpusTextInfo> <http://purl.org/net/def/metashare#CorpusTextNgramInfo> <http://purl.org/net/def/metashare#CorpusVideoInfo> <http://purl.org/net/def/metashare#LanguageDescriptionImageInfo> <http://purl.org/net/def/metashare#LanguageDescriptionTextInfo> <http://purl.org/net/def/metashare#LanguageDescriptionVideoInfo> <http://purl.org/net/def/metashare#LexicalConceptualResourceAudioInfo> <http://purl.org/net/def/metashare#LexicalConceptualResourceImageInfo> <http://purl.org/net/def/metashare#LexicalConceptualResourceTextInfo> <http://purl.org/net/def/metashare#LexicalConceptualResourceVideoInfo>)
              ] ;
      rdfs:label "información de dominio"@es , "domain info"@es ;
      rdfs:range
              [ a       owl:Class ;
                owl:unionOf (<http://purl.org/net/def/metashare#DomainInfo>)
              ] .

<http://purl.org/net/def/metashare#Thesaurus>
      a       owl:Class ;
      rdfs:label "thesaurus"@en , "tesauro"@es ;
      rdfs:subClassOf <http://purl.org/net/def/metashare#LexicalConceptualResourceInfo> .

<http://purl.org/net/def/metashare#textClassificationInfo>
      a       owl:ObjectProperty ;
      rdfs:comment "Groups together information on text type/genre of the resource"@en ;
      rdfs:domain
              [ a       owl:Class ;
                owl:unionOf (<http://purl.org/net/def/metashare#CorpusTextInfo> <http://purl.org/net/def/metashare#CorpusTextNgramInfo>)
              ] ;
      rdfs:range
              [ a       owl:Class ;
                owl:unionOf (<http://purl.org/net/def/metashare#TextClassificationInfo>)
              ] .

<http://purl.org/net/def/metashare#languageScript>
      a       owl:DatatypeProperty ;
      rdfs:comment "Specifies the writing system used to represent the language in form of a four letter code as it is defined in ISO-15924"@en ;
      rdfs:domain <http://purl.org/net/def/metashare#LanguageInfo> ;
      rdfs:range xsd:string .

<http://purl.org/net/def/metashare#creationModeDetails>
      a       owl:DatatypeProperty ;
      rdfs:domain
              [ a       owl:Class ;
                owl:unionOf (<http://purl.org/net/def/metashare#CorpusAudioInfo> <http://purl.org/net/def/metashare#CorpusImageInfo> <http://purl.org/net/def/metashare#CorpusTextInfo> <http://purl.org/net/def/metashare#CorpusTextNgramInfo> <http://purl.org/net/def/metashare#CorpusTextNumericalInfo> <http://purl.org/net/def/metashare#CorpusVideoInfo> <http://purl.org/net/def/metashare#LanguageDescriptionImageInfo> <http://purl.org/net/def/metashare#LanguageDescriptionInfo> <http://purl.org/net/def/metashare#LanguageDescriptionTextInfo> <http://purl.org/net/def/metashare#LanguageDescriptionVideoInfo> <http://purl.org/net/def/metashare#LexicalConceptualResourceInfo>)
              ] .

<http://purl.org/net/def/metashare#licenseCategory>
      a       owl:ObjectProperty ;
      rdfs:domain <http://purl.org/net/def/metashare#License> ;
      rdfs:label "categoría de licencia"@es , "license category"@en ;
      rdfs:range <http://purl.org/net/def/metashare#LicenseCategory> .

<http://purl.org/net/def/metashare#WordList>
      a       owl:Class ;
      rdfs:label "lista de palabras"@es , "word list"@en ;
      rdfs:subClassOf <http://purl.org/net/def/metashare#LexicalConceptualResourceInfo> .

<http://purl.org/net/def/metashare#mimeType>
      a       owl:DatatypeProperty ;
      rdfs:comment "The mime-type of the resource which is a formalized specifier for the format included or a mime-type that the tool/service accepts; value to be taken from a subset of the official mime types of the Internet Assigned Numbers Authority (http://www.iana.org/)"@en ;
      rdfs:domain
              [ a       owl:Class ;
                owl:unionOf (<http://purl.org/net/def/metashare#InputInfo> <http://purl.org/net/def/metashare#OutputInfo>)
              ] ;
      rdfs:range xsd:string .

rdf:langString
      a       rdfs:Datatype .

<http://purl.org/net/def/metashare#LanguageDescriptionInfo>
      a       owl:Class ;
      rdfs:comment "Groups together information on language descriptions (grammars)."@en ;
      rdfs:label "language description info"@en , "información de las gramáticas"@es .

<http://purl.org/net/def/metashare#documentInfo>
      a       owl:ObjectProperty ;
      rdfs:domain <http://purl.org/net/def/metashare#Documentation> ;
      rdfs:label "información de la documentación"@es , "document info"@en ;
      rdfs:range <http://purl.org/net/def/metashare#DocumentInfo> .

<http://purl.org/net/def/metashare#lexicalConceptualResourceType>
      a       owl:ObjectProperty ;
      rdfs:domain <http://purl.org/net/def/metashare#LexicalConceptualResourceInfo> ;
      rdfs:label "tipo de recurso léxico conceptual"@es , "lexical conceptual resource type"@en .

<http://purl.org/net/def/metashare#characterEncoding>
      a       owl:ObjectProperty ;
      rdfs:comment "The name of the character encoding used in the resource or accepted by the tool/service"@en ;
      rdfs:domain
              [ a       owl:Class ;
                owl:unionOf (<http://purl.org/net/def/metashare#CharacterEncodingInfo> <http://purl.org/net/def/metashare#InputInfo> <http://purl.org/net/def/metashare#OutputInfo>)
              ] ;
      rdfs:label "codificación de caracteres"@es , "character encoding"@en ;
      rdfs:range
              [ a       owl:Class ;
                owl:unionOf (<http://purl.org/net/def/metashare#CharacterEncoding>)
              ] .

<http://purl.org/net/def/metashare#LanguageDescriptionType>
      a       owl:Class ;
      rdfs:comment "The type of the language description"@en ;
      rdfs:label "language description type"@en , "tipo de gramática"@es .

dct:replaces
      a       owl:AnnotationProperty .

<http://purl.org/net/def/metashare#telephoneNumber>
      a       owl:DatatypeProperty ;
      rdfs:domain
              [ a       owl:Class ;
                owl:unionOf (<http://purl.org/net/def/metashare#Organization> <http://purl.org/net/def/metashare#Person>)
              ] .

<http://purl.org/net/def/metashare#LexicalConceptualResourceInfo>
      a       owl:Class ;
      rdfs:comment "Groups together information specific to lexical/conceptual resources."@en ;
      rdfs:label "lexical conceptual resource info"@en , "información del recurso léxico conceptual"@es .

<http://purl.org/net/def/metashare#organizationName>
      a       owl:DatatypeProperty ;
      rdfs:domain <http://purl.org/net/def/metashare#Organization> .

<http://purl.org/net/def/metashare#lingualityType>
      a       owl:ObjectProperty ;
      rdfs:comment "Indicates whether the resource includes one, two or more languages"@en ;
      rdfs:domain
              [ a       owl:Class ;
                owl:unionOf (<http://purl.org/net/def/metashare#CorpusAudioInfo> <http://purl.org/net/def/metashare#CorpusImageInfo> <http://purl.org/net/def/metashare#CorpusTextInfo> <http://purl.org/net/def/metashare#CorpusTextNgramInfo> <http://purl.org/net/def/metashare#CorpusVideoInfo> <http://purl.org/net/def/metashare#LanguageDescriptionImageInfo> <http://purl.org/net/def/metashare#LanguageDescriptionTextInfo> <http://purl.org/net/def/metashare#LanguageDescriptionVideoInfo> <http://purl.org/net/def/metashare#LexicalConceptualResourceAudioInfo> <http://purl.org/net/def/metashare#LexicalConceptualResourceImageInfo> <http://purl.org/net/def/metashare#LexicalConceptualResourceTextInfo> <http://purl.org/net/def/metashare#LexicalConceptualResourceVideoInfo>)
              ] ;
      rdfs:label "clasificación por número de lenguas"@es , "linguality type"@en ;
      rdfs:range
              [ a       owl:Class ;
                owl:unionOf (<http://purl.org/net/def/metashare#LingualityType>)
              ] .

<http://purl.org/net/def/metashare#languageVarietyName>
      a       owl:DatatypeProperty ;
      rdfs:comment "The name of the language variety that occurs in the resource or is supported by a tool/service"@en ;
      rdfs:domain
              [ a       owl:Class ;
                owl:unionOf (<http://purl.org/net/def/metashare#InputInfo> <http://purl.org/net/def/metashare#LanguageVarietyInfo> <http://purl.org/net/def/metashare#OutputInfo>)
              ] ;
      rdfs:range xsd:string .

<http://purl.org/net/def/metashare#licensor>
      a       owl:ObjectProperty ;
      rdfs:domain <http://purl.org/net/def/metashare#LicenceInfo> ;
      rdfs:label "licenciador"@es , "licensor"@en ;
      rdfs:range <http://purl.org/net/def/metashare#Actor> .

<http://purl.org/net/def/metashare#validationInfo>
      a       owl:ObjectProperty ;
      rdfs:domain <http://purl.org/net/def/metashare#LanguageResource> .

<http://purl.org/net/def/metashare#languageName>
      a       owl:DatatypeProperty ;
      rdfs:comment "A human understandable name of the language that is used in the resource or supported by the tool/service; an autocompletion mechanism with values from the ISO 639 is provided in the editor, but the values can be subsequently edited for further specification (according to the IETF BCP47 guidelines)"@en ;
      rdfs:domain
              [ a       owl:Class ;
                owl:unionOf (<http://purl.org/net/def/metashare#DocumentInfo> <http://purl.org/net/def/metashare#InputInfo> <http://purl.org/net/def/metashare#LanguageInfo> <http://purl.org/net/def/metashare#MetadataInfo> <http://purl.org/net/def/metashare#OutputInfo>)
              ] ;
      rdfs:range xsd:string .

<http://purl.org/net/def/metashare#ClassificationInfo>
      a       owl:Class ;
      rdfs:label "información de la clasificación"@es , "classification info"@en .

<http://purl.org/net/def/metashare#domain>
      a       owl:DatatypeProperty ;
      rdfs:comment "Specifies the application domain of the resource or the tool/service"@en ;
      rdfs:domain <http://purl.org/net/def/metashare#DomainInfo> ;
      rdfs:range xsd:string .

<http://purl.org/net/def/metashare#samplesLocation>
      a       owl:DatatypeProperty ;
      rdfs:domain <http://purl.org/net/def/metashare#LanguageResource> .

<http://purl.org/net/def/metashare#linguisticInformation>
      a       owl:ObjectProperty ;
      rdfs:comment "A more detailed account of the linguistic information contained in the lexicalConceptualResource"@en ;
      rdfs:domain <http://purl.org/net/def/metashare#LexicalConceptualResourceInfo> ;
      rdfs:label "linguistic information"@en , "información lingüística"@es ;
      rdfs:range <http://purl.org/net/def/metashare#LinguisticInformation> .

<http://purl.org/net/def/metashare#Actor>
      a       owl:Class ;
      rdfs:comment "Used to bring persons and organizations (in whatever role they may have with regard to the resource, e.g., resource creator, IPR holder, etc.)"@en ;
      rdfs:label "actor"@en , "actor"@es ;
      owl:equivalentClass <http://xmlns.com/foaf/0.1/Actor> .

<http://purl.org/net/def/metashare#CorpusVideoInfo>
      a       owl:Class ;
      rdfs:comment "Groups together information on the video component of a corpus."@en , "información de los componentes audivisuales del corpus"@es ;
      rdfs:label "Corpus video info"@en , "información de los vídeos del corpus"@es .

<http://purl.org/net/def/metashare#textGenre>
      a       owl:DatatypeProperty ;
      rdfs:subPropertyOf <http://purl.org/net/def/metashare#genre> .

<http://purl.org/net/def/metashare#LexicalConceptualResource>
      a       owl:Class ;
      rdfs:label "lexical conceptual resource"@en , "recurso léxico conceptual"@es ;
      rdfs:subClassOf <http://purl.org/net/def/metashare#LanguageResource> ;
      owl:equivalentClass
              [ a       owl:Restriction ;
                owl:onProperty <http://purl.org/net/def/metashare#lexicalConceptualResourceInfo> ;
                owl:someValuesFrom <http://purl.org/net/def/metashare#LexicalConceptualResourceInfo>
              ] .

<http://purl.org/net/def/metashare#ToolService>
      a       owl:Class ;
      rdfs:label "herramientas y servicios"@es , "tool service"@en ;
      rdfs:subClassOf <http://purl.org/net/def/metashare#LanguageResource> .

<http://purl.org/net/def/metashare#externalRef>
      a       owl:DatatypeProperty ;
      rdfs:domain <http://purl.org/net/def/metashare#LexicalConceptualResourceInfo> .

<http://purl.org/net/def/metashare#SizeUnit>
      a       owl:Class ;
      rdfs:comment "Specifies the unit that is used when providing information on the size of the resource or of resource parts."@en ;
      rdfs:label "size unit"@en , "unidad de medida del tamaño"@es .

<http://purl.org/net/def/metashare#theoreticModel>
      a       owl:DatatypeProperty ;
      rdfs:domain
              [ a       owl:Class ;
                owl:unionOf (<http://purl.org/net/def/metashare#AnnotationInfo> <http://purl.org/net/def/metashare#LanguageDescriptionInfo> <http://purl.org/net/def/metashare#LexicalConceptualResourceInfo>)
              ] .
